examples/Wrappers.dfy
@@ -60,7 +60,7 @@ module {:options "--function-syntax:4"} Demo {
   // Sometimes we want to go from Option to Result:
   method FindName(m: MyMap<string, string>) returns (res: Result<string, string>) {
     // Will return a default error message in case of None:
-    res := m.Get("name").ToResult();
+    res := m.Get("name").ToResult("'name' not found");
     // We can also match on the option to write a custom error:
     match m.Get("name")
     case Some(n) => res := Success(n);
@@ -165,12 +165,31 @@ module {:options "--function-syntax:4"} Demo {
 
     // Dynamically test whether the string is at least 5 characters long, and return a failure if not.
     // If we pass this line, Dafny can now assume that the string is long enough.
-    :- Need(|contents| >= 5, "File contents not long enough.");
+    :- Need<string>(|contents| >= 5, "File contents not long enough.");
 
     // Now we can get the character
     var c := contents[4];
 
     return Success(c);
+  }
+
+  // For a method that returns an Outcome, use Outcome.Need
+  method whatIsCharacterFive'(fs: MyFilesystem, fromPath: string) returns (res: Outcome<string>)
+    modifies fs
+  {
+
+    // Get a string that we can't reason about statically
+    var contents: string := *;
+
+    // Dynamically test whether the string is at least 5 characters long, and return a failure if not.
+    // If we pass this line, Dafny can now assume that the string is long enough.
+    :- Outcome.Need(|contents| >= 5, "File contents not long enough.");
+
+    // Now we can get the character
+    var c := contents[4];
+    // and do other stuff
+
+    return Pass;
   }
 
   method Main() {
